Coq/expose_decoupled.v
@@ -10,6 +10,264 @@ Require Import List.
 Require Import CpdtTactics.
 Require Import Coq.Logic.FunctionalExtensionality.
 
+Inductive has_access_to : config -> addr -> addr -> Prop :=
+| acc_eq  : forall σ α, has_access_to σ α α
+| acc_fld : forall σ α1 o f α2, mapp σ α1 = Some o ->
+                           flds o f = Some (v_addr α2) ->
+                           has_access_to σ α1 α2
+| acc_contn : forall χ ϕ ψ α1 x α2 s, ⌊ this ⌋ (χ, ϕ::ψ) ≜ (v_addr α1) ->
+                                 ⌊ x ⌋ (χ, ϕ::ψ) ≜ v_addr α2 ->
+                                 contn ϕ = c_stmt s ->
+                                 in_stmt x s ->
+                                 has_access_to (χ, ϕ::ψ) α1 α2.
+
+Hint Constructors has_access_to : chainmail_db.
+
+Ltac acc_auto :=
+  match goal with
+  | [ |- has_access_to _ ?α ?α] =>
+    apply acc_eq
+  | [ H : ~ has_access_to _ ?α ?α |- _] =>
+    contradiction H; acc_auto
+  | [ Hmap : mapp ?σ ?α1 = Some ?o,
+      Hfld : flds ?o ?f = Some (v_addr ?α2) |- has_access_to ?σ ?α1 ?α2] =>
+    eapply acc_fld; eauto
+  | [ Hmap : ?χ ?α1 = Some ?o,
+      Hfld : flds ?o ?f = Some (v_addr ?α2) |- has_access_to (?χ, _) ?α1 ?α2] =>
+    eapply acc_fld; eauto
+  | [ Hthis : ⌊ this ⌋ (?χ, ?ϕ::?ψ) ≜ (v_addr ?α1),
+      Hint : ⌊ ?x ⌋ (?χ, ?ϕ::?ψ) ≜ (v_addr ?α2),
+      Hcontn : contn ?ϕ = c_stmt ?s,
+      Hin : in_stmt ?x ?s |- has_access_to ?σ ?α1 ?α2] =>
+    eapply acc_contn; eauto
+  end.
+
+Lemma meth_call :
+  forall M σ1 σ2, M ∙ σ1 ⤳ σ2 ->
+             forall χ ϕ1 ψ1, σ1 = (χ, ϕ1::ψ1) ->
+                        forall x y m β s, contn ϕ1 = c_stmt (s_stmts (s_meth x y m β) s) ->
+                                     forall α1 α2, ~ has_access_to σ1 α1 α2 ->
+                                              has_access_to σ2 α1 α2 ->
+                                              ⌊ y ⌋ σ1 ≜ (v_addr α1) /\
+                                              (exists p, (β ∘ (mapp σ1)) p = Some (v_addr α2)) /\
+                                              (forall α, ⌊ this ⌋ σ1 ≜ (v_addr α) ->
+                                                    (has_access_to σ1 α α2)).
+Proof.
+  intros M σ1 σ2 Hred;
+    inversion Hred; intros; subst;
+      simpl_crush;
+      match goal with
+      | [Ha : contn ?ϕ = _,
+              Hb : contn ?ϕ = _ |- _] =>
+        rewrite Ha in Hb; inversion Hb; subst
+      end.
+
+  match goal with
+  | [H : has_access_to _ _ _ |- _] =>
+    inversion H; subst
+  end;
+    try acc_auto.
+    - repeat map_rewrite; simpl in *.
+      match goal with
+      | [H : ~ has_access_to _ _ _ |- _] =>
+        contradiction H
+      end.
+      acc_auto.
+    - repeat split; intros; simpl in *.
+      + repeat map_rewrite; simpl in *.
+        match goal with
+        | [H : c_stmt ?s1 = c_stmt ?s2 |- _] =>
+          inversion H; subst
+        end.
+        destruct (eq_dec α α1); subst; auto.
+        inversion H9; simpl in *; subst.
+        simpl_crush; simpl in *; crush.
+
+      + inversion H10; subst; simpl in *; simpl_crush; simpl in *.
+        destruct (eq_dec x this); subst;
+          [interpretation_rewrite;
+           crush|].
+        unfold update, t_update in H7;
+          eq_auto;
+          eauto.
+
+      + assert (Hex : exists p, (β ∘ (mapp (χ0, ϕ1::ψ1))) p = Some (v_addr α2)).
+        * inversion H10; subst; simpl in *; simpl_crush; simpl in *.
+          destruct (eq_dec x this); subst;
+            [interpretation_rewrite;
+             crush|].
+          unfold update, t_update in H8;
+            eq_auto;
+            eauto.
+        * let H := fresh in
+          destruct Hex as [p H];
+            simpl in H;
+            let x' := fresh "x" in
+            destruct (partial_map_dec p β) as [Hsome|Hnone];
+              [destruct Hsome as [x' Htmp]; rewrite Htmp in *
+              |rewrite Hnone in H; inversion H];
+              unfold mapp in H;
+              repeat map_rewrite; simpl in *;
+                apply acc_contn with (x:=x')(s:=(s_stmts (s_meth x0 y0 m0 β) s0));
+                auto.
+          eapply int_x; simpl; eauto.
+          apply in_stmts_1.
+          apply in_meth_3.
+          eauto.
+Qed.
+
+Ltac interpretation_auto :=
+  match goal with
+  | [|- ⌊ ?x ⌋ (?χ,?ϕ::?ψ) ≜ ?v] =>
+    match goal with
+    | [|- ⌊ x ⌋ (χ,ϕ::nil) ≜ v] => fail 1
+    | _ => idtac
+    end;
+    rewrite interpretation_x_cons; eauto
+  | [H : ⌊ ?x ⌋ (?χ,?ϕ::?ψ) ≜ ?v |- _] =>
+    notHyp (⌊ x ⌋ (χ,ϕ::nil) ≜ v);
+    rewrite interpretation_x_cons in H; eauto
+  end.
+
+Lemma classOf_cons :
+  forall x χ ϕ ψ C, classOf x (χ, ϕ::ψ) C <->
+               classOf x (χ, ϕ::nil) C.
+Proof.
+  intros x χ ϕ ψ C; split;
+    intros Hclass;
+    inversion Hclass;
+    subst;
+    eapply cls_of; eauto;
+      interpretation_auto.
+Qed.
+
+Ltac classOf_auto :=
+  match goal with
+  | [|- classOf ?x (?χ, ?ϕ::?ψ) ?C] =>
+    match goal with
+    | [|- classOf x (χ,ϕ::nil) C] => fail 1
+    | _ => idtac
+    end;
+    rewrite classOf_cons; eauto
+  | [H : classOf ?x (?χ,?ϕ::?ψ) ?C |- _] =>
+    notHyp (classOf x (χ,ϕ::nil) C);
+    rewrite classOf_cons in H; eauto
+  end.
+               
+
+Lemma stack_append_reduction_equiv :
+  forall M σ1 σ2, M ∙ σ1 ⤳ σ2 ->
+             forall ψ, M ∙ (σ1 ◁ ψ) ⤳ (σ2 ◁ ψ).
+Proof.
+  intros M σ1 σ2 Hred;
+    induction Hred;
+    intros;
+    subst;
+    unfold stack_append;
+    simpl.
+
+  - eapply r_mth; eauto.
+    eapply interpretation_x_append in H2; eauto.
+
+  - eapply r_vAssgn with (C:=C); eauto;
+      repeat classOf_auto;
+      repeat interpretation_auto.
+
+  - eapply r_fAssgn; eauto;
+      repeat interpretation_auto;
+      repeat classOf_auto.
+
+  - eapply r_new; eauto.
+
+  - eapply r_ret1; eauto.
+    repeat interpretation_auto.
+
+  - eapply r_ret2; eauto.
+    repeat interpretation_auto.
+Qed.
+
+Hint Resolve stack_append_reduction_equiv : loo_db.
+Hint Rewrite stack_append_reduction_equiv : loo_db.
+
+Lemma stack_append_reductions_equiv :
+  forall M σ1 σ2, reductions M σ1 σ2 ->
+             forall ψ, reductions M (σ1 ◁ ψ) (σ2 ◁ ψ).
+Proof.
+  intros M σ1 σ2 Hred ψ;
+    induction Hred;
+    eauto with loo_db.
+Qed.
+
+Hint Resolve stack_append_reduction_equiv : loo_db.
+Hint Rewrite stack_append_reduction_equiv : loo_db.
+Print reduction.
+Lemma return_from_method_block_1 :
+  forall M σ1 σ2, reductions M σ1 σ2 ->
+             σ_wf σ1 ->
+             forall σ3, M ∙ σ2 ⤳ σ3 ->
+                   forall χ1 ϕ1 χ2 ϕ2 ψ2 x,
+                     σ1 = (χ1, ϕ1::nil) ->
+                     σ2 = (χ2, ϕ2::ψ2) ->
+                     contn ϕ2 = (c_stmt (s_rtrn x)) ->
+                     (exists χ3 ϕ3 y z m β s α2 α3 v,
+                         σ3 = (χ3, ϕ3::nil) /\
+                         contn ϕ1 = c_stmt (s_stmts (s_meth y z m β) s) /\
+                         contn ϕ3 = c_stmt s /\
+                         ⌊ this ⌋ σ1 ≜ (v_addr α3) /\
+                         ⌊ this ⌋ σ3 ≜ (v_addr α3) /\
+                         ⌊ z ⌋ σ1 ≜ (v_addr α2) /\
+                         ⌊ this ⌋ σ2 ≜ (v_addr α2) /\
+                         vMap ϕ2 x = Some v /\
+                         vMap ϕ3 = (update y v (vMap ϕ1))) \/
+                     (exists χ' ϕ' ψ' χ3 ϕ3 y z m β s α2 α3 v,
+                         reductions M σ1 (χ', ϕ'::ψ') /\
+                         σ3 = (χ3, ϕ3::ψ') /\
+                         contn ϕ' = c_stmt (s_stmts (s_meth y z m β) s) /\
+                         contn ϕ3 = c_stmt s /\
+                         ⌊ this ⌋ (χ', ϕ'::ψ') ≜ (v_addr α3) /\
+                         ⌊ this ⌋ σ3 ≜ (v_addr α3) /\
+                         ⌊ z ⌋ (χ', ϕ'::ψ') ≜ (v_addr α2) /\
+                         ⌊ this ⌋ σ2 ≜ (v_addr α2) /\
+                         vMap ϕ2 x = Some v /\
+                         vMap ϕ3 = (update y v (vMap ϕ'))).
+Proof.
+  intros M σ1 σ2 Hred;
+    induction Hred;
+    intros;
+    subst.
+
+  - match goal with
+    | [H : ?M ∙ (_, ?ϕ2::_) ⤳ ?σ3,
+           Hcontn : contn ?ϕ2 = c_stmt (s_rtrn _) |- _] =>
+      inversion H; subst
+    end;
+      repeat simpl_crush;
+      match goal with
+      | [ Ha : contn ?ϕ = _,
+               Hb : contn ?ϕ = _ |- _] =>
+        rewrite Ha in Hb; inversion Hb; subst
+      end.
+    left.
+    inversion H; subst;
+      repeat simpl_crush.
+    crush;
+      simpl in *.
+    remember ({| vMap := vMap ϕ0; contn := c_hole y s |}) as ϕ'.
+    exists χ, (update_ϕ_contn (update_ϕ_map ϕ' y α) (c_stmt s)), y, y0, m, ps, s, α0.
+    admit.
+
+  - admit.
+    
+Admitted.
+  
+
+Lemma reduce_access_change :
+  forall M σ1 σ2, M ∙ σ1 ⤳ σ2 ->
+             forall α1 α2, ~ has_access_to σ1 α1 α2 ->
+                      has_access_to σ2 α1 α2 ->
+                      
+                                    
+
 Module ExposeExample.
 
   (** #<h3># Safe example: #</h3># *)
